theories/analysis/RealExp.ec
@@ -1,0 +1,202 @@
+(* -------------------------------------------------------------------- *)
+require import Fun Int IntExtra Real RealExtra StdRing StdOrder.
+(*---*) import RField RealOrder.
+
+(* -------------------------------------------------------------------- *)
+op exp : real -> real.
+op ln  : real -> real.
+
+axiom exp0     : exp 0%r = 1%r.
+axiom expD     : forall (x y : real), exp (x + y) = exp x * exp y.
+axiom exp_mono : forall (x y : real), (exp x <= exp y) <=> (x <= y).
+axiom exp_gt0  : forall x, 0%r < exp x.
+axiom ln_le0   : forall x, x <= 0%r => ln x = 0%r.
+
+axiom lnK  : forall x, ln (exp x) = x.
+axiom expK : forall x, 0%r < x => exp (ln x) = x.
+
+op log (a : real) = fun x => ln x / ln a.
+
+op log10 x = log 10%r x.
+op log2  x = log  2%r x.
+
+op e : real = exp 1%r.
+
+axiom ge2_e : 2%r <= e.
+axiom lt3_e : e < 3%r.
+
+lemma nosmt e_boundW : 2%r <= e <= 3%r.
+proof. by rewrite ge2_e /= ltrW ?lt3_e. qed.
+
+lemma nosmt e_gt0 : 0%r < e.
+proof. by apply/(@ltr_le_trans 2%r)/ge2_e. qed.
+
+lemma nosmt e_ge0 : 0%r <= e.
+proof. by apply/ltrW/e_gt0. qed.
+
+lemma nosmt exp_neq0 x : exp x <> 0%r.
+proof. by have := (exp_gt0 x); rewrite ltr_neqAle eq_sym => []. qed.
+
+lemma nosmt ln0 : ln 0%r = 0%r.
+proof. by rewrite ln_le0. qed.
+
+lemma nosmt inj_exp : injective exp.
+proof. by apply/mono_inj/exp_mono. qed.
+
+lemma nosmt expN (x : real) : exp (- x) = inv (exp x).
+proof.
+apply/(mulfI _ (exp_neq0 x)); rewrite -expD addrN exp0.
+by rewrite mulrV // exp_neq0.
+qed.
+
+lemma nosmt exp_mono_ltr (x y : real): (exp x < exp y) <=> (x < y).
+proof. by apply/lerW_mono/exp_mono. qed.
+
+lemma nosmt ln_mono (x y : real):
+  0%r < x => 0%r < y => (ln x <= ln y) <=> (x <= y).
+proof. by move=> gt0x gt0y; rewrite -exp_mono !expK. qed.
+
+lemma nosmt ln_mono_ltr (x y : real):
+  0%r < x => 0%r < y => (ln x < ln y) <=> (x < y).
+proof. by move=> gt0x gt0y; rewrite -exp_mono_ltr !expK. qed.
+
+lemma nosmt ln1 : ln 1%r = 0%r.
+proof. by rewrite -exp0 lnK. qed.
+
+lemma nosmt lnM (x y : real) : 0%r < x => 0%r < y =>
+  ln (x * y) = ln x + ln y.
+proof.
+move=> gt0x gt0y; apply/inj_exp; rewrite expK ?pmulr_lgt0 //.
+by rewrite expD !expK.
+qed.
+
+lemma nosmt lnV (x : real) : 0%r < x => ln (inv x) = -(ln x).
+proof. by move=> gt0x; apply/inj_exp; rewrite expN !expK ?invr_gt0. qed.
+
+lemma nosmt ln_ge0 (x:real): 1%r <= x => 0%r <= ln x.
+proof. by move=> ge1x; rewrite -exp_mono exp0 expK // (ltr_le_trans 1%r). qed.
+
+(* -------------------------------------------------------------------- *)
+op ( ^ ) (x a : real) =
+  if x <= 0%r then b2r (a = 0%r) else exp (a * ln x).
+
+(* -------------------------------------------------------------------- *)
+lemma rpowE (x a : real) : 0%r < x => x^a = exp (a * ln x).
+proof. by rewrite /(^) ltrNge => ->. qed.
+
+lemma nosmt rpoweE (a : real) : e^a = exp a.
+proof. by rewrite rpowE 1:e_gt0 // lnK mulr1. qed.
+
+(* -------------------------------------------------------------------- *)
+lemma rpow0 x : x^0%r = 1%r.
+proof. by rewrite /(^); case: (x <= 0%r)=> // _; rewrite mul0r exp0. qed.
+
+lemma rpow1 x : 0%r < x => x^1%r = x.
+proof. by move=> gt0x; rewrite rpowE // mul1r expK. qed.
+
+(* -------------------------------------------------------------------- *)
+lemma rpow0r n : 0%r^n = b2r (n = 0%r).
+proof. by rewrite /(^) lerr /=. qed.
+
+lemma rpow1r n : 1%r^n = 1%r.
+proof. by rewrite rpowE // ln1 mulr0 exp0. qed.
+
+(* -------------------------------------------------------------------- *)
+lemma rpoweK (x : real) : 0%r < x => e^(ln x) = x.
+proof. by rewrite rpoweE; apply/expK. qed.
+
+lemma rpowe_mono (n m:real): e^n <= e^m <=> n <= m.
+proof. by rewrite !rpoweE exp_mono. qed.
+
+lemma rpowe_hmono (n m:real): n <= m => e^n <= e^m.
+proof. by rewrite rpowe_mono. qed.
+
+(* -------------------------------------------------------------------- *)
+lemma rpow_gt0 (x n : real): 0%r < x => 0%r < x^n.
+proof. by move/rpowE=> ->; apply/exp_gt0. qed.
+
+lemma rpow_ge0 (x n : real): 0%r <= x => 0%r <= x^n.
+proof.
+rewrite ler_eqVlt => [<-|/rpow_gt0 /(_ n) /ltrW] //.
+by rewrite rpow0r; case: (n = 0%r).
+qed.
+
+(* -------------------------------------------------------------------- *)
+lemma rpowD (x n m : real) : 0%r < x => x^(n + m) = x^n * x^m.
+proof. by move=> gt0x; rewrite !rpowE // mulrDl expD. qed.
+
+lemma rpowM (x n m : real) : 0%r < x => x^(n * m) = (x ^ n) ^ m.
+proof. by move=> gt0x; rewrite !rpowE ?exp_gt0 // lnK mulrCA mulrA. qed.
+
+lemma rpowMr (x y n : real) :
+  0%r < x => 0%r < y => (x * y)^n = x^n * y^n.
+proof.
+move=> gt0x gt0y; rewrite !rpowE 1:pmulr_rgt0 //.
+by rewrite lnM // mulrDr expD.
+qed.
+
+lemma rpowVr (x n : real) : 0%r < x => (inv x)^n = inv (x^n).
+proof. by move=> gt0x; rewrite !rpowE ?invr_gt0 ?lnV // mulrN expN. qed.
+
+lemma rpowMVr (x y n : real):
+  0%r < x => 0%r < y => (x/y)^n = x^n/y^n.
+proof. by move=> gt0x gt0y; rewrite !divrE rpowMr ?invr_gt0 // rpowVr. qed.
+
+lemma rpow_int x n : 0%r <= x => x^(n%r) = x^n.
+proof. admit. qed.
+
+(* -------------------------------------------------------------------- *)
+lemma rpowe_gt0 (x : real): 0%r < e^x.
+proof. by rewrite rpoweE exp_gt0. qed.
+
+lemma rpowe_ge0 (x : real): 0%r <= e^x.
+proof. by rewrite rpoweE ltrW ?exp_gt0. qed.
+
+(* -------------------------------------------------------------------- *)
+lemma nosmt rpoweM (x y : real): e^(x * y) = (e^x)^y.
+proof. by rewrite rpowM // e_gt0. qed.
+
+(* -------------------------------------------------------------------- *)
+lemma nosmt rpow_mono (x y n : real):
+     0%r < n => 0%r < x => 0%r < y
+  => (x^n <= y^n) <=> (x <= y).
+proof.
+move=> gt0n gt0x gt0y; rewrite !rpowE //.
+by rewrite exp_mono ler_pmul2l // ln_mono.
+qed.
+
+lemma nosmt rpow_hmono (x y n : real):
+  0%r <= n => 0%r <= x <= y => x ^ n <= y ^ n.
+proof.
+rewrite ler_eqVlt=> [<-|gt0n]; first by rewrite !rpow0 lerr.
+case; rewrite ler_eqVlt=> [<-|gt0x] ge0y.
+  move: gt0n; rewrite rpow0r ltr_neqAle eq_sym.
+  by case=> [-> _]; apply/rpow_ge0.
+by rewrite rpow_mono //; apply/(ltr_le_trans x).
+qed.
+
+lemma nosmt rpowr_hmono (x n m : real) :
+  1%r <= x => 0%r <= n <= m => x^n <= x^m.
+proof.
+move=> ge1x [ge0n lenm]; have ge0m: 0%r <= m by apply/(ler_trans n).
+rewrite !rpowE 1,2:(ltr_le_trans 1%r) // exp_mono.
+by apply/ler_wpmul2r=> //; apply/ln_ge0.
+qed.
+
+lemma nosmt le1Dx_rpowe (x : real): 0%r <= x => 1%r+x <= e^x.
+proof. admitted.
+
+(* -------------------------------------------------------------------- *)
+require import StdBigop.
+(*---*) import Bigreal BRA BRM.
+
+lemma exp_sum (P : 'a -> bool) (F : 'a -> real) s:
+  exp (BRA.big P F s) = BRM.big P (fun a => exp (F a)) s.
+proof.
+elim: s => [|x s ih]; rewrite !(big_nil, big_cons) ?exp0 //.
+by case: (P x)=> // Px; rewrite expD ih.
+qed.
+
+lemma rpowe_sum (P : 'a -> bool) (F : 'a -> real) s:
+  e^(BRA.big P F s) = BRM.big P (fun a => e^(F a)) s.
+proof. by rewrite rpoweE exp_sum; apply/eq_bigr=> x _ /=; rewrite rpoweE. qed.
